theory/x64DecodeProof.thy
@@ -1,0 +1,119 @@
+theory x64DecodeProof
+imports
+  Main
+  rBPFCommType rBPFSyntax
+  x64Assembler x64Disassembler
+begin
+
+lemma [simp]: "l @ [a] = l_bin \<Longrightarrow> l_bin!(length l) = a" by fastforce
+lemma [simp]: "l @ [a, b] = l_bin \<Longrightarrow> l_bin!(length l) = a" by fastforce  
+lemma [simp]: "l @ [a, b, c] = l_bin \<Longrightarrow> l_bin!(length l) = a" by fastforce
+lemma [simp]: "l @ [a, b, c, d] = l_bin \<Longrightarrow> l_bin!(length l) = a" by fastforce
+lemma [simp]: "l @ [a, b, c, d, e] = l_bin \<Longrightarrow> l_bin!(length l) = a" by fastforce
+
+lemma [simp]: "l @ [a, b] = l_bin \<Longrightarrow> l_bin!(length l + 1) = b"
+  by (metis One_nat_def nth_Cons_0 nth_Cons_Suc nth_append_length_plus)
+lemma [simp]: "l @ [a, b, c] = l_bin \<Longrightarrow> l_bin!(length l + 1) = b"
+  by (metis One_nat_def nth_Cons_0 nth_Cons_Suc nth_append_length_plus)
+lemma [simp]: "l @ [a, b, c, d] = l_bin \<Longrightarrow> l_bin!(length l + 1) = b"
+  by (metis One_nat_def nth_Cons_0 nth_Cons_Suc nth_append_length_plus)
+lemma [simp]: "l @ [a, b, c, d, e] = l_bin \<Longrightarrow> l_bin!(length l + 1) = b"
+  by (metis One_nat_def nth_Cons_0 nth_Cons_Suc nth_append_length_plus)
+
+lemma [simp]: "l @ [a, b] = l_bin \<Longrightarrow> l_bin!(Suc (length l)) = b"
+  by (metis One_nat_def add_diff_cancel_right' not_add_less2 nth_Cons_0 nth_Cons_Suc nth_append plus_1_eq_Suc)
+lemma [simp]: "l @ [a, b, c] = l_bin \<Longrightarrow> l_bin!(Suc (length l)) = b"
+  by (metis One_nat_def add_diff_cancel_right' not_add_less2 nth_Cons_0 nth_Cons_Suc nth_append plus_1_eq_Suc)
+lemma [simp]: "l @ [a, b, c, d] = l_bin \<Longrightarrow> l_bin!(Suc (length l)) = b"
+  by (metis One_nat_def add_diff_cancel_right' not_add_less2 nth_Cons_0 nth_Cons_Suc nth_append plus_1_eq_Suc)
+lemma [simp]: "l @ [a, b, c, d, e] = l_bin \<Longrightarrow> l_bin!(Suc (length l)) = b"
+  by (metis One_nat_def add_diff_cancel_right' not_add_less2 nth_Cons_0 nth_Cons_Suc nth_append plus_1_eq_Suc)
+
+lemma [simp]: "l @ [a, b, c] = l_bin \<Longrightarrow> l_bin!(length l + 2) = c"
+  by (metis One_nat_def Suc_1 nth_Cons_0 nth_Cons_Suc nth_append_length_plus)
+lemma [simp]: "l @ [a, b, c, d] = l_bin \<Longrightarrow> l_bin!(length l + 2) = c"
+  by (metis One_nat_def Suc_1 nth_Cons_0 nth_Cons_Suc nth_append_length_plus)
+lemma [simp]: "l @ [a, b, c, d, e] = l_bin \<Longrightarrow> l_bin!(length l + 2) = c"
+  by (metis One_nat_def Suc_1 nth_Cons_0 nth_Cons_Suc nth_append_length_plus)
+
+
+lemma [simp]: "l @ [a, b, c] = l_bin \<Longrightarrow> l_bin!(Suc (Suc (length l))) = c"
+  by (metis Cons_eq_appendI One_nat_def add_Suc_right append_Nil length_append list.size(3) list.size(4) nth_append_length nth_append_length_plus plus_1_eq_Suc)
+lemma [simp]: "l @ [a, b, c, d] = l_bin \<Longrightarrow> l_bin!(Suc (Suc (length l))) = c"
+  by (metis Cons_eq_appendI One_nat_def add_Suc_right append_Nil length_append list.size(3) list.size(4) nth_append_length nth_append_length_plus plus_1_eq_Suc)
+lemma [simp]: "l @ [a, b, c, d, e] = l_bin \<Longrightarrow> l_bin!(Suc (Suc (length l))) = c"
+  by (metis Cons_eq_appendI One_nat_def add_Suc_right append_Nil length_append list.size(3) list.size(4) nth_append_length nth_append_length_plus plus_1_eq_Suc)
+
+lemma [simp]: "l @ [a, b, c, d] = l_bin \<Longrightarrow> l_bin!(length l + 3) = d"
+  by force
+lemma [simp]: "l @ [a, b, c, d, e] = l_bin \<Longrightarrow> l_bin!(length l + 3) = d"
+  by force
+
+
+lemma [simp]: "l @ [a, b, c, d] = l_bin \<Longrightarrow> l_bin!(Suc (Suc (Suc (length l)))) = d"
+  by (metis One_nat_def Suc3_eq_add_3 add_diff_cancel_right' last.simps last_conv_nth length_Cons list.discI list.size(3) not_add_less2 nth_append)
+lemma [simp]: "l @ [a, b, c, d, e] = l_bin \<Longrightarrow> l_bin!(Suc (Suc (Suc (length l)))) = d"
+  by (metis Suc3_eq_add_3 add.commute nth_Cons_0 nth_Cons_Suc nth_append_length_plus numeral_3_eq_3)
+
+lemma [simp]: "l @ [a, b, c, d, e] = l_bin \<Longrightarrow> l_bin!(length l + 4) = e"
+  by force
+
+lemma [simp]: "l @ [a, b, c, d, e] = l_bin \<Longrightarrow> l_bin!(Suc (Suc (Suc (Suc (length l))))) = e"
+  by (metis Nil_is_append_conv One_nat_def Suc_1 add_2_eq_Suc' add_Suc_right diff_Suc_1' last.simps last_appendR last_conv_nth length_Cons length_append list.discI list.size(3))
+
+lemma [simp]: "l @ [a] = l_bin \<Longrightarrow> length l_bin - length l = 1" by fastforce
+lemma [simp]: "l @ [a, b] = l_bin \<Longrightarrow> length l_bin - length l = 2" by fastforce  
+lemma [simp]: "l @ [a, b, c] = l_bin \<Longrightarrow> length l_bin - length l = 3" by fastforce
+lemma [simp]: "l @ [a, b, c, d] = l_bin \<Longrightarrow> length l_bin - length l = 4" by fastforce
+lemma [simp]: "l @ [a, b, c, d, e] = l_bin \<Longrightarrow> length l_bin - length l = 5" by fastforce
+
+
+lemma x64_encode_decode_consistency:
+  "x64_encode ins l = Some l_bin \<Longrightarrow> x64_decode (length l) l_bin = Some (length l_bin - length l, ins)"
+  apply (unfold x64_encode_def)
+  apply (cases ins; simp_all)
+
+  subgoal for src dst
+  \<comment> \<open> Pmovl_rr \<close> 
+    apply (unfold Let_def)
+    apply (cases "construct_rex_to_u8 False (and (u8_of_ireg dst) 8 \<noteq> 0) False (and (u8_of_ireg src) 8 \<noteq> 0) = 0", simp_all add: construct_rex_to_u8_def construct_modsib_to_u8_def)
+    subgoal by (cases src; cases dst; auto simp add: x64_decode_def bitfield_insert_u8_def Let_def ireg_of_u8_def)
+    subgoal by (cases src; cases dst; auto simp add: x64_decode_def bitfield_insert_u8_def Let_def ireg_of_u8_def)
+    done
+
+  subgoal for dst src
+  \<comment> \<open> Pmovq_rr \<close> 
+    apply (unfold Let_def construct_rex_to_u8_def construct_modsib_to_u8_def)
+    subgoal by (cases src; cases dst; auto simp add: x64_decode_def bitfield_insert_u8_def Let_def ireg_of_u8_def)
+    done
+
+  subgoal for src dst chunk
+  \<comment> \<open> Pmov_rm \<close> 
+    apply (cases dst, simp)
+    subgoal for rd rs ro
+      apply (cases rd, simp_all)
+      subgoal for rd1
+        apply (cases rs, simp_all)
+        apply (cases "rd1 = ireg.R11 \<and> ro = 0", simp_all add: Let_def)
+        apply (unfold Let_def construct_rex_to_u8_def construct_modsib_to_u8_def)
+        apply (cases chunk; cases src; auto simp add: x64_decode_def bitfield_insert_u8_def Let_def ireg_of_u8_def)
+        done
+      done
+    done
+
+ \<comment> \<open> 
+    apply (cases src)
+    subgoal
+      apply (cases dst)
+      subgoal
+        apply (auto simp add: bitfield_insert_u8_def Let_def u8_of_bool_def)
+        apply (unfold x64_decode_def Let_def)
+        apply simp
+        value "unsigned_bitfield_extract_u8 4 4 (8)"
+
+        apply (auto simp add: bitfield_insert_u8_def Let_def ireg_of_u8_def)
+
+    subgoal by (cases src; cases dst; auto simp add: x64_decode_def bitfield_insert_u8_def Let_def ireg_of_u8_def)
+ \<close> 
+  done
+end
